Uppaal_Networks/UPPAAL_Asm_AbsInt.thy
@@ -1,0 +1,24 @@
+theory UPPAAL_Asm_AbsInt
+  imports UPPAAL_Asm
+begin
+
+type_synonym 'a ainstr = "'a * instr" \<comment> \<open>Instruction with state before it is executed\<close>
+type_synonym 'a aprogram = "addr \<Rightarrow> (('a ainstr) option)"
+
+fun annot_all :: "program \<Rightarrow> 'a \<Rightarrow> 'a aprogram" where
+  "annot_all prog v addr =
+    (case prog addr of
+        Some instr \<Rightarrow> Some (v, instr)
+      | None \<Rightarrow> None)"
+
+(* this probably makes no sense: *)
+fun collect_step :: "state set aprogram \<Rightarrow> state \<Rightarrow> state set aprogram" where
+  "collect_step prog entry pc =
+    (let ainstr = (prog pc) in
+    case ainstr of
+        Some (astates, instr) \<Rightarrow>
+          let instates = if state_pc entry = pc then astates \<union> {entry} else astates in
+          undefined
+      | None \<Rightarrow> None)"
+
+end
