Uppaal_Networks/UPPAAL_Asm_ControlFlow.thy
@@ -1,0 +1,123 @@
+theory UPPAAL_Asm_ControlFlow
+  imports UPPAAL_Asm
+begin
+
+text \<open>
+  Analysis of a program with respect to successor and predecessor addresses for each contained
+  instruction. Predecessors are necessary for abstract interpretation to know from where to
+  "pull forward" the states.
+\<close>
+
+type_synonym succs = "addr \<Rightarrow> addr set"
+type_synonym predecs = "addr \<Rightarrow> addr set"
+
+fun successors :: "program \<Rightarrow> succs" where
+  "successors prog pc =
+    (case prog pc of
+        Some (JMPZ jmp) \<Rightarrow> {jmp, pc + 1}
+      | Some HALT       \<Rightarrow> {}
+      | None            \<Rightarrow> {}
+      | _               \<Rightarrow> {pc + 1})"
+
+
+lemma stack2: obtains "s = []" | "\<exists>a ss. s = a # ss" by (meson list.exhaust) 
+lemma stack3: obtains "s = []" | "\<exists>a. s = a # []" | "\<exists>a b ss. s = a # b # ss"
+  by (meson remdups_adj.cases) (* TODO: this rule here makes no sense *)
+
+lemma successors_complete:
+  assumes
+    "Some instr = ((prog::program) pc)"
+    "step instr (pc, st, m, f, rs) = Some (rpc, rst, rm, rf, rrs)"
+  shows "rpc \<in> successors prog pc"
+proof (cases "instr")
+case (JMPZ x1)
+  from this assms show ?thesis sorry
+next
+  case ADD
+  from assms(2) this have nextpc: "rpc = pc + 1" by (cases "st" rule: stack3) auto
+  from ADD assms(1) have "prog pc = Some ADD" by simp
+  from this nextpc ADD show ?thesis by auto
+next
+  case NOT
+  from assms(2) this have nextpc: "rpc = pc + 1" by (cases "st" rule: stack2) auto
+  from NOT assms(1) have "prog pc = Some NOT" by simp
+  from this nextpc show ?thesis by auto
+next
+  case AND
+  from assms(2) this have nextpc: "rpc = pc + 1"
+  proof (cases "st" rule: stack2)
+    case 2
+    then obtain b ss where "st = b # ss" by blast
+    from assms(2) AND this show ?thesis by (cases "b = 0 \<or> b = 1") auto
+  qed auto
+  from AND assms(1) have "prog pc = Some AND" by simp
+  from this nextpc show ?thesis by auto
+next
+  case LT
+  from assms(2) this have nextpc: "rpc = pc + 1" by (cases "st" rule: stack3) auto
+  from LT assms(1) have "prog pc = Some LT" by simp
+  from this nextpc show ?thesis by auto
+next
+  case LE
+  from assms(2) this have nextpc: "rpc = pc + 1" by (cases "st" rule: stack3) auto
+  from LE assms(1) have "prog pc = Some LE" by simp
+  from this nextpc show ?thesis by auto
+next
+  case EQ
+  from assms(2) EQ have nextpc: "rpc = pc + 1" by (cases "st" rule: stack3) auto
+  from EQ assms(1) have "prog pc = Some EQ" by simp
+  from this nextpc show ?thesis by auto
+next
+  case (PUSH x8)
+  from assms(2) this have nextpc: "rpc = pc + 1" by auto
+  from PUSH assms(1) have "prog pc = Some (PUSH x8)" by simp
+  from this nextpc show ?thesis by auto
+next
+  case POP
+  from assms(2) POP have nextpc: "rpc = pc + 1" by (cases "st" rule: stack2) auto
+  from POP assms(1) have "prog pc = Some POP" by simp
+  from this nextpc show ?thesis by auto
+next
+  case (LID x10)
+  from assms(2) LID have nextpc: "rpc = pc + 1" by auto
+  from LID assms(1) have "prog pc = Some (LID x10)" by simp
+  from this nextpc show ?thesis by auto
+next
+  case STORE
+  from assms(2) STORE have nextpc: "rpc = pc + 1"
+  proof (cases "st" rule: stack3)
+    case 3
+    from this obtain v r sst where "st = v # r # sst" by blast
+    from assms(2) STORE this show ?thesis by (cases "r \<ge> 0") auto
+  qed auto
+  from STORE assms(1) have "prog pc = Some STORE" by simp
+  from this nextpc show ?thesis by auto
+next
+  case (STOREI x121 x122)
+  from assms(2) STOREI have nextpc: "rpc = pc + 1" by auto
+  from STOREI assms(1) have "prog pc = Some (STOREI x121 x122)" by simp
+  from this nextpc show ?thesis by auto
+next
+  case COPY
+  from assms(2) COPY have nextpc: "rpc = pc + 1" by auto
+  from COPY assms(1) have "prog pc = Some COPY" by simp
+  from this nextpc show ?thesis by auto
+next
+  case CALL
+  (* This cannot work, CALL is indirect *)
+  then show ?thesis sorry
+next
+  case RETURN
+  then show ?thesis sorry
+next
+  case HALT
+  then show ?thesis sorry
+next
+  case (STOREC x171 x172)
+  then show ?thesis sorry
+next
+  case (SETF x18)
+  then show ?thesis sorry
+qed
+
+end
